\providecommand{\main}{../main2}
\documentclass[\main/main.tex]{subfiles}
\graphicspath{{../images2/}}
\begin{document}
% \begin{frame}{}
%     \begin{align}
%         R(L_•⊗L_∘) = (L_∘⊗L_•)R
%     \end{align}
%     \begin{align}
%         R(T_•⊗T_∘) = (T_∘⊗T_•)R
%     \end{align}
%     \begin{align}
%         [τ_•, τ_∘] = 0
%     \end{align}
%     \begin{align*}
%         &
%         \det \mqty(
%             c_∘c_• & 0 & a_∘a_•-b_∘b_•
%             \\
%             c_∘a_• & -c_∘b_• & a_∘c_•
%             \\
%             a_∘c_• & -b_∘c_• & c_∘a_•
%         )
%         \\ &
%         =c_∘c_•(-a_•b_•c_∘^2+a_∘b_∘c_•^2) + c_∘c_•(a_∘a-b_∘b)(-a_•b_∘+a_∘b_•)
%         = 0.
%     \end{align*}
%     \begin{align}
%         \f{a_∘²+b_∘²-c_∘²}{2a_∘b_∘}
%         = \f{a_•²+b_•²-c_•²}{2a_•b_•}
%         ≡ Δ_∘-Δ_• = 0
%     \end{align}
%     \begin{align}
%         Δ = Δ_∘ = Δ_•
%     \end{align}
% \end{frame}
% \begin{frame}{}
%     \begin{align}
%         \begin{cases}
%             a = \sin(λ+2η)
%             \\
%             b = \sin λ
%             \\
%             c = \sin(2η)
%         \end{cases}
%     \end{align}
%     \begin{align}
%         Δ = \f{a²+b²-c²}{2ab} = \cos(2η)
%     \end{align}
%     \begin{align}
%         (λ_∘+2η)λ_• - λ_∘(λ_•+2η) = 2ηλ
%     \end{align}
%     \begin{align}
%         λ = λ_• - λ_∘
%     \end{align}
% \end{frame}
% \begin{frame}
%     \begin{align}
%         a_∘b_• - b_∘a_• = cb
%     \end{align}
%     \begin{align}
%         \sin(λ_∘+2η)\sin(λ_•) - \sin(λ_∘)\sin(λ_•+2η)
%         = c\sin λ
%     \end{align}
%     \begin{align}
%         &
%         (Δ\sin λ_∘+c\cos λ_∘)\sin λ_•
%         - (Δ\sin λ_•+c\cos λ_•)\sin λ_∘
%         \\ &
%         = c \sin λ_•\cos λ_∘ - c \cos λ_• \sin λ_∘
%         \\ &
%         = c \sin(λ_• - λ_∘)
%     \end{align}
%     \begin{align}
%         c² \cos(λ_∘+λ_•) + cΔ \sin(λ_∘+λ_•)
%         = c\sin(λ_∘+λ_•+2η)
%     \end{align}
% \end{frame}
% \begin{frame}{}
% \begin{align}
% \f{1}{2}\M(
%     (a+b)+(a-b)σ^z & 2cσ^- \\
%     2cσ^+ & (a+b)-(a-b)σ^z
% )
% \end{align}
% \begin{align}
%     \f{1}{2}\M(
%         (a+b)+(a-b)σ^z & 2cσ^- \\
%         2cσ^+ & (a+b)-(a-b)σ^z
%     ){\k{↑}}
%     = \M(
%         a\k{↑} & c\k{↓} \\
%         0 & b\k{↑}
%     )
% \end{align}
% \end{frame}
% \begin{frame}{}
% \begin{align}
%     L(λ) = \M(
%         a(λ-η)π_↑+b(λ-η)π_↓ & c(λ-η)σ^-\\
%         c(λ-η)σ^+ & a(λ-η)π_↑-b(λ-η)π_↓
%     )
% \end{align}
% \begin{align}
%     π_↑ = \f{1+σ^z}{2}, \q
%     π_↓ = \f{1-σ^z}{2}
% \end{align}
% \begin{align}
%     \f{b(λ₁-λ)}{c(λ₁-λ)}α(λ₁) + \f{b(λ-λ₁)}{c(λ-λ₁)}δ(λ₁) = 0
% \end{align}
% \begin{align}
%     \f{α(λ₁)}{δ(λ₁)} = \Q(\f{a(λ₁-η)}{b(λ₁-η)})^N = 1
% \end{align}
% \begin{align}
%     \f{a(λ₁-η)}{b(λ₁-η)} = e^{ik₁},
%     \q k₁ ∈ \f{2π}{Na}ℤ
% \end{align}
% \begin{align}
%     e^{ik₁} = \f{λ₁+η}{λ₁-η}
% \end{align}
% \end{frame}
% \begin{frame}{}
% \begin{align}
%     B(λ)|0⟩
% \end{align}
% \begin{align}
%     L₁(λ)L₂(λ)\k{↑}₁\k{↑}₂
%     &
%     =\M(a\k{↑}₁&c\k{↓}₁\\0&b\k{↑}₁)
%         \M(a\k{↑}₂&c\k{↓}₂\\0&b\k{↑}₂)
%     \\ &
%     =\M(a²\k{↑↑} & ac\k{↑↓}+cb\k{↓↑} \\
%         0        & b²\k{↑↑} )
% \end{align}
% \begin{align}
%     L₁(λ)L₂(λ)L₃(λ)\k{↑}₁\k{↑}₂\k{↑}₃
%     &
%     =\M(a²\k{↑↑} & ac\k{↑↓}+cb\k{↓↑} \\
%         0        & b²\k{↑↑} )
%         \M(a\k{↑}₃&c\k{↓}₃\\0&b\k{↑}₃)
%     \\ &
%     =\M(a³\k{↑↑↑} & a²c\k{↑↑↓}+acb\k{↑↓↑}+cb²\k{↓↑↑}\\
%        0 & b³\k{↑↑↑})
% \end{align}
% \end{frame}
% \begin{frame}{}
% \begin{gather}
%     B(λ)|0⟩
%     = ∑_{n=1}^{N} a^{n-1} c b^{N-n} |⋯↓ₙ⋯⟩
%     \\
%     |⋯↓ₙ⋯⟩ = |{↑}⟩₁⋯|{↑}⟩ₙ₋₁|{↓}⟩ₙ|{↑}⟩ₙ₊₁⋯|{↑}⟩_N
% \end{gather}
% \begin{align}
%     |k₁⟩
%     = ∑_{n=1}^{N} e^{ik₁n} |⋯↓ₙ⋯⟩,
%     \q
%     k₁ ∈ \f{2π}{N}ℤ
% \end{align}
% \end{frame}
% \begin{frame}{}
% このうち使う交換関係は3つだけで、1行目4列目、1行目3列目、2行目4列目に注目すると、
% \begin{gather}
%     BB' = B'B
%     \\
%     aBA' = cA'B + bB'A
%     \\
%     bBD' + cDB' = aB'D
% \end{gather}
% \begin{align}
%     &
%     [B(λ),B(μ)] = 0
%     \\ &
%     A(λ)B(μ)
%     = \f{a(μ-λ)}{c(μ-λ)}B(λ)A(μ)
%     - \f{b(μ-λ)}{c(μ-λ)}B(μ)A(λ)
%     \\ &
%     D(λ)B(μ)
%     = \f{a(λ-μ)}{c(λ-μ)}B(μ)D(λ)
%     - \f{b(λ-μ)}{c(λ-μ)}B(λ)D(μ)
% \end{align}
% \end{frame}
% \begin{frame}{}
%     \begin{align}
%         &
%         [B(λ),B(μ)] = 0
%         \\ &
%         A(λ)B(μ)
%         = f(μ-λ)B(λ)A(μ)
%         - g(μ-λ)B(μ)A(λ)
%         \\ &
%         D(λ)B(μ)
%         = f(λ-μ)B(μ)D(λ)
%         + g(λ-μ)B(λ)D(μ)
%     \end{align}
%     \begin{align}
%         &
%         A(λ)B(λ₁)|0⟩
%         = \f{a(λ₁-λ)}{c(λ₁-λ)} B(λ₁)α(λ)|0⟩ 
%         - \f{b(λ₁-λ)}{c(λ₁-λ)} B(λ)α(λ₁)|0⟩
%         \\ &
%         D(λ)B(λ₁)|0⟩
%         = \f{a(λ-λ₁)}{c(λ-λ₁)}B(λ₁)δ(λ)|0⟩
%         - \f{b(λ-λ₁)}{c(λ-λ₁)}B(λ)δ(λ₁)|0⟩
%     \end{align}
% \end{frame}

\begin{frame}{}
\begin{align}
    α(λ)B(λ₁)⋯B(λ_M)|0⟩, \q
    α(λᵢ)B(λ₁)⋯\overbrace{B(λ)}^i⋯B(λ_M)|0⟩
\end{align}
\begin{align}
    \Q[\f{a(λ₁-λ)}{c(λ₁-λ)}B(λ₁)A(λ)
    - \f{b(λ₁-λ)}{c(λ₁-λ)}B(λ)A(λ₁)]B(λ₂)⋯B(λ_M)|0⟩
\end{align}
\begin{align*}
    -\f{b(λ₁-λ)}{c(λ₁-λ)}B(λ)\Q[\f{a(λ₂-λ₁)}{c(λ₂-λ₁)}B(λ₂)A(λ₁)
    - \f{b(λ₂-λ₁)}{c(λ₂-λ₁)}B(λ₁)A(λ₂)]B(λ₃)⋯B(λ_M)|0⟩
\end{align*}
\begin{align}
    - \f{b(λ₁-λ)}{c(λ₁-λ)} \Q{∏_{i≠1}\f{a(λᵢ-λ₁)}{c(λᵢ-λ₁)}} α(λ₁)B(λ)B(λ₂)⋯B(λ_M)|0⟩
\end{align}
\begin{align}
    - \f{b(λⱼ-λ)}{c(λⱼ-λ)} \Q{∏_{i≠j}\f{a(λᵢ-λⱼ)}{c(λᵢ-λⱼ)}} α(λⱼ)B(λ₁)⋯\overbrace{B(λ)}^j⋯B(λ_M)|0⟩
\end{align}

\end{frame}
\begin{frame}{}
\begin{align}
    - \f{b(λ-λⱼ)}{c(λ-λⱼ)} \Q{∏_{i≠j}\f{a(λⱼ-λᵢ)}{c(λⱼ-λᵢ)}} δ(λⱼ)B(λ₁)⋯\overbrace{B(λ)}^j⋯B(λ_M)|0⟩
\end{align}
\begin{align}
    α(λⱼ)\f{b(λⱼ-λ)}{c(λⱼ-λ)} ∏_{i≠j}\f{a(λᵢ-λⱼ)}{c(λᵢ-λⱼ)}
    + δ(λⱼ)\f{b(λ-λⱼ)}{c(λ-λⱼ)} ∏_{i≠j}\f{a(λⱼ-λᵢ)}{c(λⱼ-λᵢ)} = 0
\end{align}
\begin{align}
    \f{α(λⱼ)}{δ(λⱼ)} = ∏_{i≠j}\f{a(λⱼ-λᵢ)}{a(λᵢ-λⱼ)}
\end{align}
\begin{align}
    \Q(\f{a(λⱼ-η)}{b(λⱼ-η)})^N = ∏_{i≠j}\f{a(λⱼ-λᵢ)}{a(λᵢ-λⱼ)}
\end{align}
\begin{align}
    \Q(\f{λⱼ+η}{λⱼ-η})^N
    = (-1)^{M-1}∏_{i≠j}\f{λⱼ-λᵢ+2η}{λⱼ-λᵢ-2η}
\end{align}
\begin{align}
    Λ(λ;λ₁,…,λ_M) = α(λ) ∏_{i=1}^M \f{a(λᵢ-λ)}{c(λᵢ-λ)}
    + δ(λ) ∏_{i=1}^M \f{a(λ-λᵢ)}{c(λ-λᵢ)}
\end{align}
\end{frame}
\begin{frame}{}
\begin{align}
    Lₙ(λ)|{↑}⟩ₙ = \M(a(λ)|{↑}⟩ₙ & c(λ)|{↓}⟩ₙ \\ 0 & b(λ)|{↑}⟩ₙ)
\end{align}
\begin{align}
    T(λ)|0⟩ = L₁(λ)⋯L_N(λ)|0⟩ = \M(a(λ)^N|0⟩ & * \\ 0 & b(λ)^N|0⟩)
\end{align}
\begin{align}
    α(λ) ≡ a(λ)^N, \q δ(λ) ≡ b(λ)^N
\end{align}
\begin{align}
    τ(λ)|0⟩ = (A(λ)+D(λ))|0⟩ = (α(λ) + δ(λ))|0⟩
\end{align}
\begin{align}
    α(λ₁) = δ(λ₁)
\end{align}
\begin{align}
    [A(λ)+D(λ)]B(λ₁)⋯B(λ_M)|0⟩ ∝ B(λ₁)⋯B(λ_M)|0⟩
\end{align}
\end{frame}
\begin{frame}{}
\begin{align}
    L_{n,α}
    &
    = \M(
        a&0&0&0\\
        0&b&c&0\\
        0&c&b&0\\
        0&0&0&a
    )
    = \M(
        aπ_n^+ + bπ_n^- & cσ_n^- \\
        cσ_n^+ & bπ_n^+ + aπ_n^-
    )
    \\ &
    = \f{a+b}{2}1_α1_n+\f{a-b}{2}σ_α^zσ_n^z+\f{c}{2}(σ_α^xσ_n^x+σ_α^yσ_n^y)
\end{align}
\begin{align}
    σ^x = \M(0&1\\1&0),\q
    σ^y = \M(0&-i\\i&0),\q
    σ^z = \M(1&0\\0&-1).
\end{align}
\begin{align}
    π^+ = \f{1+σ^z}{2},
    \q
    π^- = \f{1-σ^z}{2}.
\end{align}
\begin{align}
    σ^+ = \f{σ^x + iσ^y}{2},
    \q
    σ^- = \f{σ^x - iσ^y}{2}.
\end{align}
\end{frame}
\begin{frame}{}
\begin{align}
    R(λ)
    = \M(
        \sinh(λ+2η) & 0                & 0            & 0 \\
        0           &  e^{-λ}\sinh(2η) & \sinh λ      & 0 \\
        0           & \sinh λ          & e^λ\sinh(2η) & 0 \\
        0           & 0                & 0            & \sinh(λ+2η)
    )
\end{align}
\begin{align}
    R ≡ \lim_{λ→∞} 2e^{-λ-η}R(λ)
    = \M(
        e^η & 0      & 0             & 0 \\
        0   & 0      & e^{-η}        & 0 \\
        0   & e^{-η} & e^{η}-e^{-3η} & 0 \\
        0   & 0      & 0             & e^η
    )
\end{align}
\begin{align}
    R
    = \M(
        A & 0   & 0       & 0 \\
        0 & 0   & A⁻¹     & 0 \\
        0 & A⁻¹ & A - A⁻³ & 0 \\
        0 & 0   & 0       & A
    ), \q
    A = e^η
\end{align}
\end{frame}
\begin{frame}{}
\begin{align}
    A = e^η
\end{align}
\begin{align}
    \graph[scale=0.1]{R.png}= \M(
        A & 0   & 0       & 0 \\
        0 & 0   & A⁻¹     & 0 \\
        0 & A⁻¹ & A - A⁻³ & 0 \\
        0 & 0   & 0       & A
    )
\end{align}
\begin{align}
    \graph[scale=0.05]{RR^-1.png} = 1
\end{align}
\begin{align}
    \graph[scale=0.1]{R^-1.png}=\M(
        A⁻¹ & 0      & 0 & 0 \\
        0   & A⁻¹-A³ & A & 0 \\
        0   & A      & 0 & 0 \\
        0   & 0      & 0 & A⁻¹
    )
\end{align}
\end{frame}
\begin{frame}{}
\begin{align}
    \graph[scale=0.1]{R.png}~
    =A~\graph[scale=0.1]{1.png}~
    +A^{-1}~\graph[scale=0.1]{fi.png}~
\end{align}
\begin{align}
    \graph[scale=0.1]{fi.png}~
    = A~\graph[scale=0.1]{R.png}~
    - A²~\graph[scale=0.1]{1.png}~
    = \M(
        0&0  &0 &0\\
        0&-A²&1 &0\\
        0&1  &-A⁻²&0\\
        0&0  &0 &0
    )
\end{align}
\begin{align}
    \graph[scale=0.1]{o.png} = \tr~\graph[scale=0.1]{fi.png}~
    = -A²-A⁻²
\end{align}
\begin{align}
    \graph[scale=0.1]{twist.png} = -A³\M(1&0\\0&1)
\end{align}
\end{frame}
\end{document}